- Added some initial content to ITP - Proved the HP predicates correspond to prescriptions

theories/theories/utp_prescr.thy
@@ -8,6 +8,7 @@ header {* UTP Prescriptions *}
 
 theory utp_prescr
 imports utp_designs
+begin
 
 definition "HP(P) = `P \<lhd> ok \<rhd> \<not> ok'`"
 
@@ -30,22 +31,61 @@ lemma HP_form_equiv2:
   assumes "`p[false/okay]` = `\<not> ok'`"
   shows "p is HP"
 using assms
-apply (utp_poly_tac)
-apply (safe, simp_all)
-apply (drule_tac x="b" in spec)
-apply (simp)
-apply (subgoal_tac "b(okay :=\<^sub>* False) = b")
-apply (simp)
-defer
-apply (drule_tac x="b" in spec, simp)
-apply (rule ccontr)
-apply (subgoal_tac "b = b(okay :=\<^sub>* False)")
-apply (simp)
-apply (metis (full_types) TypeUSound_bool binding_upd_drop_ty pvaux_MkPVAR)
-by (metis (full_types) TypeUSound_bool binding_upd_drop_ty pvaux_MkPVAR)
+  apply (utp_poly_tac)
+  apply (safe, simp_all)
+  apply (drule_tac x="b" in spec)
+  apply (simp)
+  apply (subgoal_tac "b(okay :=\<^sub>* False) = b")
+  apply (simp)
+  defer
+  apply (drule_tac x="b" in spec, simp)
+  apply (rule ccontr)
+  apply (subgoal_tac "b = b(okay :=\<^sub>* False)")
+  apply (simp)
+  apply (metis (full_types) TypeUSound_bool binding_upd_drop_ty pvaux_MkPVAR)+
+done
   
 theorem HP_form_equiv:
   "`P[false/okay]` = `\<not> ok'` \<longleftrightarrow> P is HP"
   by (metis HP_form_equiv1 HP_form_equiv2)
+
+definition PrescrP :: 
+  "'a WF_PREDICATE \<Rightarrow> 
+   'a WF_PREDICATE \<Rightarrow> 
+   'a WF_PREDICATE" (infixr "\<parallel>-" 60) where
+"P \<parallel>- Q = `(ok \<and> P \<Rightarrow> ok') \<and> (ok' \<Rightarrow> Q \<and> ok)`"
+
+syntax
+  "_upred_prescr" :: "upred \<Rightarrow> upred \<Rightarrow> upred" (infixr "\<parallel>-" 30)
+
+translations
+  "_upred_prescr p q" == "CONST PrescrP p q"
+
+declare PrescrP_def [eval, evalp]
+
+theorem PrescrP_HP:
+  "P \<parallel>- Q is HP"
+  apply (unfold HP_form_equiv[THEN sym])
+  apply (simp add:PrescrP_def usubst typing defined)
+done
+
+theorem HP_as_PrescrP:
+  assumes "P is HP"
+  shows "P = `\<not> P\<^bsup>tf\<^esup> \<parallel>- P\<^bsup>tt\<^esup>`"
+proof -
+  have "`(\<not> P\<^bsup>tf\<^esup> \<parallel>- P\<^bsup>tt\<^esup>)[true/okay]` = `P[true/okay]`"
+    apply (simp add:PrescrP_def usubst typing defined)
+    apply (utp_poly_auto_tac)
+  sorry
+
+  moreover from assms have "`(\<not> P\<^bsup>tf\<^esup> \<parallel>- P\<^bsup>tt\<^esup>)[false/okay]` = `P[false/okay]`"
+    by (simp add:PrescrP_def usubst typing defined HP_form_equiv[THEN sym])
+
+  ultimately show ?thesis
+    apply (subst BoolType_pvaux_cases[of okay])
+    apply (simp_all add:closure typing)
+  done
+qed
+
 
 end
